spec/abstract/KHeap_A.thy
@@ -45,6 +45,16 @@ where
 section "TCBs"
 
 definition
+  get_tcb :: "obj_ref \<Rightarrow> 'z::state_ext state \<Rightarrow> tcb option"
+where
+  "get_tcb tcb_ref state \<equiv>
+   case kheap state tcb_ref of
+      None      \<Rightarrow> None
+    | Some kobj \<Rightarrow> (case kobj of
+        TCB tcb \<Rightarrow> Some tcb
+      | _       \<Rightarrow> None)"
+
+definition
   thread_get :: "(tcb \<Rightarrow> 'a) \<Rightarrow> obj_ref \<Rightarrow> ('a,'z::state_ext) s_monad"
 where
   "thread_get f tptr \<equiv> do
@@ -257,7 +267,71 @@ where
            Some (runnable (tcb_state tcb) \<and> (test_sc_refill_max sc_ptr s)
            \<and> \<not>in_release_q))"
 
-definition reschedule_required :: "unit det_ext_monad" where
+definition
+  get_tcb_queue :: "domain \<Rightarrow> priority \<Rightarrow> (ready_queue, 'z::state_ext) s_monad" where
+  "get_tcb_queue d prio \<equiv> do
+     queues \<leftarrow> gets ready_queues;
+     return (queues d prio)
+   od"
+
+definition
+  set_tcb_queue :: "domain \<Rightarrow> priority \<Rightarrow> ready_queue \<Rightarrow> (unit, 'z::state_ext) s_monad" where
+  "set_tcb_queue d prio queue \<equiv>
+     modify (\<lambda>es. es\<lparr> ready_queues :=
+      (\<lambda>d' p. if d' = d \<and> p = prio then queue else ready_queues es d' p)\<rparr>)"
+
+definition
+  tcb_sched_action :: "(obj_ref \<Rightarrow> obj_ref list \<Rightarrow> obj_ref list) \<Rightarrow> obj_ref  \<Rightarrow> (unit, 'z::state_ext) s_monad"
+where
+  "tcb_sched_action action thread \<equiv> do
+     d \<leftarrow> thread_get tcb_domain thread;
+     prio \<leftarrow> thread_get tcb_priority thread;
+     queue \<leftarrow> get_tcb_queue d prio;
+     set_tcb_queue d prio (action thread queue)
+   od"
+
+definition
+  tcb_sched_enqueue :: "obj_ref \<Rightarrow> obj_ref list \<Rightarrow> obj_ref list" where
+  "tcb_sched_enqueue thread queue \<equiv> if (thread \<notin> set queue) then thread # queue else queue"
+
+definition
+  tcb_sched_append :: "obj_ref \<Rightarrow> obj_ref list \<Rightarrow> obj_ref list" where
+  "tcb_sched_append thread queue \<equiv> if (thread \<notin> set queue) then queue @ [thread] else queue"
+
+definition
+  tcb_sched_dequeue :: "obj_ref \<Rightarrow> obj_ref list \<Rightarrow> obj_ref list" where
+  "tcb_sched_dequeue thread queue \<equiv> filter (\<lambda>x. x \<noteq> thread) queue"
+
+definition
+  in_release_queue :: "obj_ref \<Rightarrow> 'z::state_ext state \<Rightarrow> bool"
+where
+  "in_release_queue tcb_ptr \<equiv> \<lambda>s. tcb_ptr \<in> set (release_queue s)"
+
+definition
+  tcb_release_dequeue :: "(unit, 'z::state_ext) s_monad"
+where
+  "tcb_release_dequeue =
+    modify (\<lambda>s. s\<lparr> release_queue := tl (release_queue s), reprogram_timer := True \<rparr>)"
+
+definition
+  tcb_release_remove :: "obj_ref \<Rightarrow> (unit, 'z::state_ext) s_monad"
+where
+  "tcb_release_remove tcb_ptr = modify (release_queue_update (tcb_sched_dequeue tcb_ptr))"
+
+definition
+  set_scheduler_action :: "scheduler_action \<Rightarrow> (unit, 'z::state_ext) s_monad" where
+  "set_scheduler_action action \<equiv>
+     modify (\<lambda>es. es\<lparr>scheduler_action := action\<rparr>)"
+
+definition
+  thread_set_priority :: "obj_ref \<Rightarrow> priority \<Rightarrow> (unit, 'z::state_ext) s_monad" where
+  "thread_set_priority tptr prio \<equiv> thread_set (\<lambda>tcb. tcb\<lparr>tcb_priority := prio\<rparr>) tptr"
+
+definition
+  thread_set_domain :: "obj_ref \<Rightarrow> domain \<Rightarrow> (unit, 'z::state_ext) s_monad" where
+  "thread_set_domain tptr domain \<equiv> thread_set (\<lambda>tcb. tcb\<lparr>tcb_domain := domain\<rparr>) tptr"
+
+definition reschedule_required :: "(unit, 'z::state_ext) s_monad" where
   "reschedule_required \<equiv> do
      action \<leftarrow> gets scheduler_action;
      case action of
@@ -271,7 +345,7 @@ definition reschedule_required :: "unit det_ext_monad" where
    od"
 
 definition
-  schedule_tcb :: "obj_ref \<Rightarrow> unit det_ext_monad"
+  schedule_tcb :: "obj_ref \<Rightarrow> (unit, 'z::state_ext) s_monad"
 where
   "schedule_tcb tcb_ptr \<equiv> do
     cur \<leftarrow> gets cur_thread;
@@ -282,17 +356,15 @@ where
   od"
 
 definition
-  set_thread_state_ext :: "obj_ref \<Rightarrow> unit det_ext_monad"
+  set_thread_state_act :: "obj_ref \<Rightarrow> (unit, 'z::state_ext) s_monad"
 where
-  "set_thread_state_ext tcb_ptr \<equiv> do
+  "set_thread_state_act tcb_ptr \<equiv> do
     cur \<leftarrow> gets cur_thread;
     sched_act \<leftarrow> gets scheduler_action;
     in_release_q \<leftarrow> gets $ in_release_queue tcb_ptr;
     schedulable \<leftarrow> is_schedulable tcb_ptr in_release_q;
     when (tcb_ptr = cur \<and> sched_act = resume_cur_thread \<and> \<not>schedulable) $ set_scheduler_action choose_new_thread
   od"
-
-
 
 
 (***)
@@ -303,7 +375,7 @@ where
   "set_thread_state ref ts \<equiv> do
      tcb \<leftarrow> gets_the $ get_tcb ref;
      set_object ref (TCB (tcb \<lparr> tcb_state := ts \<rparr>));
-     do_extended_op (set_thread_state_ext ref)
+     set_thread_state_act ref
    od"
 
 definition
